Sealing: Factored out witness heaps.

theories/heap_lang/lib/sealing.v
@@ -115,12 +115,130 @@ Section instances.
 End instances.
 End intf.
 
-(** * Morris' implementation *)
+(** * Witness heaps *)
+(**
+	Both of the following proofs rely on a so-called _witness
+	heap_; that is, a ghost heap [h] sending locations [k] to
+	sealed values [v].
+*)
+(** The CMRA we need. *)
+Local Notation heap := (gmap loc val).
+Definition heapUR : ucmraT := gmapUR loc (agreeR valC).
+Class sealingG Σ := SealingG { sealing_heapG :> inG Σ (authR heapUR) }.
+
+Definition sealingΣ : gFunctors := #[ GFunctor (constRF (authR heapUR)) ].
+Instance subG_sealingΣ {Σ} : subG sealingΣ Σ → sealingG Σ.
+Proof. intros [??]%subG_inv. constructor; apply _. Qed.
+
+Module witness.
+Section witness.
+  Context `{heapG Σ, sealingG Σ}.
+
+  (** Definitions. *)
+
+  (**
+	The assertion [is_witness γ k v] represents knowledge that the
+	witness heap named [γ] sends location [k] to value [v].
+  *)
+  Definition is_witness (γ : gname) (k : loc) (v : val) : iProp Σ :=
+    own γ (◯ {[k := to_agree v]}).
+  Definition to_heap : heap → heapUR := fmap to_agree.
+  Definition witness (γ : gname) (h : heap) : iProp Σ :=
+    (own γ (● to_heap h) ∗ live (dom _ h))%I.
+
+  (** Structure *)
+
+  Global Instance is_witness_persistent γ k v :
+    PersistentP (is_witness γ k v).
+  Proof. apply _. Qed.
+  Global Instance is_witness_timeless γ k v :
+    TimelessP (is_witness γ k v).
+  Proof. apply _. Qed.
+
+  (** Ghosts *)
+
+  Lemma witness_alloc : (|==> ∃ γ, witness γ ∅)%I.
+  Proof.
+    set h := to_heap ∅.
+    iMod (own_alloc (Auth (Excl' h) h)) as (γ) "Hw"; first done.
+    iModIntro. iExists γ.
+    rewrite (auth_both_op h). iDestruct "Hw" as "[Hw _]". iFrame "Hw".
+    by rewrite dom_empty_L big_sepS_empty.
+  Qed.
+
+  Lemma is_witness_elim γ h k v :
+    witness γ h -∗ is_witness γ k v -∗ ⌜h !! k = Some v⌝.
+  Proof.
+    iIntros "[Hw _] Hk".
+    iDestruct (own_valid_2 with "Hw Hk") as %[Hinc _]%auth_valid_discrete_2.
+    iPureIntro.
+    move: Hinc. rewrite singleton_included lookup_fmap=>-[] u [].
+    case: (h !! k)=>[vh|]/=; last by move=>/option_equivE.
+    move=>Heq. apply (inj Some) in Heq. unfold_leibniz. rewrite -Heq.
+    by case/Some_included=>[/(inj to_agree) | /to_agree_included]->.
+  Qed.
+
+  Lemma is_witness_alloc' γ h k v :
+    h !! k = None →
+    own γ (● to_heap h) ==∗
+    own γ (● to_heap (<[k:=v]> h)) ∗ is_witness γ k v.
+  Proof.
+    rewrite /to_heap fmap_insert -own_op=>Hdom.
+    apply own_update, auth_update_alloc, alloc_singleton_local_update.
+    by rewrite lookup_fmap Hdom. done.
+  Qed.
+
+  Lemma is_witness_alloc γ h k v :
+    heap_ctx -∗ witness γ h -∗ fresh k ={⊤}=∗
+    ⌜h !! k = None⌝ ∗ witness γ (<[k:=v]> h) ∗ is_witness γ k v.
+  Proof.
+    iIntros "#Hh [Hw Hlive] Hk".
+    iMod (heap_mark_live with "Hh Hk Hlive") as "(Hdom&Hlive)"; first done.
+      iDestruct "Hdom" as %?%not_elem_of_dom.
+    iMod (is_witness_alloc' _ _ k v with "Hw") as "[Hw Hv]"; first done.
+    iModIntro. iFrame "% Hw Hv". rewrite dom_insert_L. by iFrame "Hlive".
+  Qed.
+
+  Lemma witness_obs γ h k v :
+    h !! k = Some v →
+    witness γ h ==∗ witness γ h ∗ is_witness γ k v.
+  Proof.
+    iIntros (Hdom) "[Hw HL]". rewrite/witness/is_witness. iFrame "HL".
+    rewrite -own_op. iApply (own_update with "Hw").
+    apply auth_frag_alloc; try apply _. apply singleton_included.
+    exists (to_agree v). split. by rewrite lookup_fmap Hdom. done.
+  Qed.
+
+  Lemma is_witness_agree γ k v1 v2 :
+    is_witness γ k v1 ∗ is_witness γ k v2 ⊢ ⌜v1 = v2⌝.
+  Proof.
+    rewrite -own_op -auth_frag_op.
+    rewrite own_valid auth_validI /= discrete_valid.
+    rewrite op_singleton singleton_valid.
+    by f_equiv=>/agree_op_inv/to_agree_inj/leibniz_equiv_iff.
+  Qed.
+
+  (** Somewhat orthogonal. *)
+  Lemma tbl_inv_insert (h : heap) k v (φ : val → iProp Σ) :
+    ([∗ map] v ∈ h, □ φ v) -∗ □ φ v -∗ [∗ map] v ∈ <[k:=v]> h, □ φ v.
+  Proof.
+    iIntros "Hinv #Hv". case Hv': (h !! k) => [v'|].
+    - rewrite (big_sepM_insert_override_2 _ _ _ v' v) //.
+      iApply "Hinv". iIntros "_". iAlways. by iFrame "Hv".
+    - rewrite big_sepM_insert //. iFrame "Hinv". iAlways. by iFrame "Hv".
+  Qed.
+End witness.
+End witness.
+
+(** * Morris' sealing implementation *)
 (**
 	Other than the typecast, this is a transliteration of Morris'
-	implementation of sealing.
+	code. We need the typecast to match our library for finite
+	maps which assumes a type of values with decidable equality
+	(here, locations).
 
-	Safe-for-space implementations exist. The sequential code
+	Safe-for-space implementations likely exist. We conjecture
+	that the sequential code
 <<
 	let r = ref None in
 	let seal x = λ _, r := Some x in
@@ -138,6 +256,8 @@ End intf.
 	(accessed in February 2017).
 *)
 Module morris_sealing.
+Import witness.
+
 Section code.
   Context {LI : LockImpl}.
 
@@ -161,15 +281,6 @@ Section code.
   |}.
 End code.
 
-(** The CMRA we need. *)
-Notation heap := (gmap loc val).
-Definition heapUR : ucmraT := gmapUR loc (agreeR valC).
-Class sealingG Σ := SealingG { sealing_heapG :> inG Σ (authR heapUR) }.
-
-Definition sealingΣ : gFunctors := #[ GFunctor (constRF (authR heapUR)) ].
-Instance subG_sealingΣ {Σ} : subG sealingΣ Σ → sealingG Σ.
-Proof. intros [??]%subG_inv. constructor; apply _. Qed.
-
 Section proof.
   Context `{heapG Σ, sealingG Σ, LI : LockImpl} (L : lock Σ).
   Implicit Types l : loc.
@@ -179,33 +290,27 @@ Section proof.
 	The table underlying the sealer-unsealer pair named [γ] sends
 	locations [k] to values satisfying the representation
 	invariant [φ]. Moreover, locations [k] arising from verified
-	applications of [unseal] are tied to a ghost heap witnessing
-	the table's assignment of a particular value [v] to [k].
+	applications of [unseal] are tied to a witness heap.
+	(Witnesses are used to prove the progressive triple for
+	unsealing.)
 
-	The table must account for locations not tracked by the ghost
-	heap because adversarial code can apply a sealed value to a
-	low-integrity value [kv]. When [kv] is a location [k], such
-	applications extend the table, but not the ghost heap.
+	The table must account for locations not tracked by the
+	witness heap because adversarial code can apply a sealed value
+	to a low-integrity value [kv]. When [kv] is a location [k],
+	such applications extend the table, but not the witness heap.
 
-	The assertion [is_witness γ k v] represents knowledge that the
-	ghost heap sends location [k] to value [v] and is used to
-	prove the progressive triple for unsealing. The resource
-	[witness γ m] ties the ghost heap to a sealer-unsealer pair
-	with table contents [m] and heap resources that ensure we can
-	allocate [is_witness γ k v] given a fresh, high location [k].
+	The resource [witness_some γ m] ties the witness heap to a
+	sealer-unsealer pair with table contents [m] and to heap
+	resources that ensure we can allocate witnesses given a fresh,
+	high location [k].
   *)
 
-  Definition is_witness (γ : gname) (k : loc) (v : val) : iProp Σ :=
-    own γ (◯ {[k := to_agree v]}).
-
-  Definition to_heap : heap → heapUR := fmap to_agree.
-  Definition witness (γ : gname) (m : heap) : iProp Σ := (
-    ∃ h, ⌜h ⊆ m⌝ ∗ own γ (● to_heap h) ∗ live (dom _ h) ∗
-    [∗ map] k↦_ ∈ h, k ↦ ()
+  Definition witness_some (γ : gname) (m : heap) : iProp Σ := (
+    ∃ h, ⌜h ⊆ m⌝ ∗ witness γ h ∗ [∗ map] k↦_ ∈ h, k ↦ ()
   )%I.
 
   Definition tbl_res (l : loc) (γ : gname) (φ : val → iProp Σ) : iProp Σ := (
-    ∃ map m, l ↦ map ∗ is_map map m ∗ witness γ m ∗
+    ∃ map m, l ↦ map ∗ is_map map m ∗ witness_some γ m ∗
     [∗ map] v ∈ m, □ φ v
   )%I.
 
@@ -239,11 +344,6 @@ Section proof.
 
   (** Structure *)
 
-  Instance is_witness_persistent γ k v : PersistentP (is_witness γ k v).
-  Proof. apply _. Qed.
-  Instance is_witness_timeless γ k v : TimelessP (is_witness γ k v).
-  Proof. apply _. Qed.
-
   Instance tbl_res_ne l γ n : Proper (ext (dist n) ==> dist n) (tbl_res l γ).
   Proof. solve_proper. Qed.
 
@@ -271,38 +371,27 @@ Section proof.
 
   (** Ghosts *)
 
-  Lemma witness_elim γ m k v :
-    witness γ m -∗ is_witness γ k v -∗ ⌜m !! k = Some v⌝.
+  Lemma witness_some_alloc : (|==> ∃ γ, witness_some γ ∅)%I.
   Proof.
-    iIntros "Hw Hk". iDestruct "Hw" as (h) "(%&Hγ&_)".
-    iDestruct (own_valid_2 with "Hγ Hk") as %[Hinc _]%auth_valid_discrete_2.
-    iPureIntro. apply (map_subseteq_spec h m); first done.
-    move: Hinc. rewrite singleton_included lookup_fmap=>-[] u [].
-    case: (h !! k)=>[vh|]/=; last by move=>/option_equivE.
-    move=>Heq. apply (inj Some) in Heq. unfold_leibniz. rewrite -Heq.
-    by case/Some_included=>[/(inj to_agree) | /to_agree_included]->.
+    iMod witness_alloc as (γ) "Hw". iModIntro. iExists γ, ∅. iFrame "Hw".
+    rewrite big_sepM_empty. by auto.
   Qed.
 
-  Lemma witness_high_alloc γ h k v :
-    h !! k = None →
-    own γ (● to_heap h) ==∗
-    own γ (● to_heap (<[k:=v]> h)) ∗ is_witness γ k v.
+  Lemma is_witness_some_elim γ m k v :
+    witness_some γ m -∗ is_witness γ k v -∗ ⌜m !! k = Some v⌝.
   Proof.
-    rewrite /to_heap fmap_insert -own_op=>Hdom.
-    apply own_update, auth_update_alloc, alloc_singleton_local_update.
-    by rewrite lookup_fmap Hdom. done.
+    iIntros "Hw Hk". iDestruct "Hw" as (h) "(%&Hw&_)".
+    iDestruct (is_witness_elim with "Hw Hk") as "%". iPureIntro.
+    by apply (map_subseteq_spec h m).
   Qed.
 
-  Lemma witness_high γ m k v :
-    heap_ctx -∗ witness γ m -∗ k ↦ () -∗ fresh k ={⊤}=∗
-    witness γ (<[k:=v]> m) ∗ is_witness γ k v.
+  Lemma is_witness_alloc_high γ m k v :
+    heap_ctx -∗ witness_some γ m -∗ k ↦ () -∗ fresh k ={⊤}=∗
+    witness_some γ (<[k:=v]> m) ∗ is_witness γ k v.
   Proof.
-    iIntros "#Hh Hw Hk Hf". iDestruct "Hw" as (h) "(%&Hγ&Hlive&Hhigh)".
-    iMod (heap_mark_live with "Hh Hf Hlive") as "(Hdom&Hlive)"; first done.
-      iDestruct "Hdom" as %?%not_elem_of_dom.
-    iMod (witness_high_alloc _ _ k v with "Hγ") as "[Hγ Hw]"; first done.
-    iModIntro. iFrame "Hw". iExists (<[k:=v]> h). iFrame "Hγ".
-    rewrite dom_insert_L. iFrame "Hlive".
+    iIntros "#Hh Hw Hk Hf". iDestruct "Hw" as (h) "(%&Hw&Hhigh)".
+    iMod (is_witness_alloc _ _ _ v with "Hh Hw Hf") as "(%&Hw&Hv)".
+    iModIntro. iFrame "Hv". iExists (<[k:=v]> h). iFrame "Hw".
     rewrite big_sepM_insert //. iFrame "Hk Hhigh".
     iPureIntro. apply map_subseteq_spec=>x vx.
     case: (decide (k = x))=>[<-|?]; first by rewrite !lookup_insert.
@@ -320,24 +409,15 @@ Section proof.
     - rewrite lookup_insert_ne //. by iApply (IH with "Hhigh Hl").
   Qed.
 
-  Lemma witness_low γ m k v :
-    witness γ m -∗ low k -∗ witness γ (<[k:=v]> m).
+  Lemma witness_some_low γ m k v :
+    witness_some γ m -∗ low k -∗ witness_some γ (<[k:=v]> m).
   Proof.
-    iIntros "Hw Hk". iDestruct "Hw" as (h) "(%&Hγ&Hlive&Hhigh)". iExists h.
+    iIntros "Hw Hk". iDestruct "Hw" as (h) "(%&Hγ&Hhigh)". iExists h.
     iDestruct (witness_low_sep with "Hhigh Hk") as "#Hdom".
       iDestruct "Hdom" as %Hdom.
-    iFrame "Hγ Hlive Hhigh". iPureIntro. apply map_subseteq_spec=>x vx.
+    iFrame "Hγ Hhigh". iPureIntro. apply map_subseteq_spec=>x vx.
     case: (decide (k = x))=>[<-|?]; first by rewrite Hdom.
     rewrite lookup_insert_ne //. by apply map_subseteq_spec.
-  Qed.
-
-  Lemma tbl_inv_insert (m : heap) k v (φ : val → iProp Σ) :
-    ([∗ map] v ∈ m, □ φ v) -∗ □ φ v -∗ [∗ map] v ∈ <[k:=v]> m, □ φ v.
-  Proof.
-    iIntros "Hinv #Hv". case Hv': (m !! k) => [v'|].
-    - rewrite (big_sepM_insert_override_2 _ _ _ v' v) //.
-      iApply "Hinv". iIntros "_". iAlways. by iFrame "Hv".
-    - rewrite big_sepM_insert //. iFrame "Hinv". iAlways. by iFrame "Hv".
   Qed.
 
   (** Properties of sealing *)
@@ -357,7 +437,7 @@ Section proof.
       iDestruct "HR" as (map m) "(Hl & Hm & Hw & #Hinv)". wp_load.
     wp_apply (map_insert_spec _ _ _ m with "Hm").
       iIntros (map') "Hm'". rewrite -wp_fupd. wp_store.
-    iMod (witness_high _ _ k v with "Hh Hw Hk Hf") as "[Hw Hkv]".
+    iMod (is_witness_alloc_high _ _ k v with "Hh Hw Hk Hf") as "[Hw Hkv]".
     iApply ("HΨ" with "[Hv Hl Hm' Hw]"); last by iApply ("HΦ" with "Hkv").
     iExists map', (<[k:=v]> m). iFrame "Hl Hm' Hw".
     by iApply (tbl_inv_insert with "Hinv Hv").
@@ -378,7 +458,7 @@ Section proof.
       iIntros (map') "Hm'". wp_store.
     iApply ("HΨ" with "[Hl Hm' Hw]"); last by iApply "HΦ"; simpl_low.
     iExists map', (<[k:=v]> m). iFrame "Hl Hm'". iSplitL.
-    - rewrite (low_val k). by iApply (witness_low with "Hw Hk").
+    - rewrite (low_val k). by iApply (witness_some_low with "Hw Hk").
     - by iApply (tbl_inv_insert with "Hinv [Hv]").
   Qed.
 
@@ -442,12 +522,8 @@ Section proof.
     {{{ v1 v2 γ, RET (v1, v2); is_seal γ v1 φ ∗ is_unseal γ v2 φ }}}.
   Proof.
     iIntros (? Φ) "#Hh HΦ". wp_lam. wp_alloc l as "Hl". wp_let.
-      rewrite -wp_fupd. set h := to_heap ∅.
-    iMod (own_alloc (Auth (Excl' h) h)) as (γh) "Hγh"; first done.
-      rewrite (auth_both_op h). iDestruct "Hγh" as "[Hγh _]".
-    iAssert (witness γh ∅) with "[Hγh]" as "Hw".
-    { iExists ∅. iFrame "Hγh".
-      rewrite dom_empty_L big_sepS_empty big_sepM_empty. by auto. }
+      rewrite -wp_fupd.
+    iMod witness_some_alloc as (γh) "Hw".
     wp_apply (make_sync_spec L _ N (tbl_res l γh φ) with "[$Hh Hl Hw]");
       first done.
     { iExists map_empty, ∅. iFrame "Hl Hw". rewrite big_sepM_empty. by auto. }
@@ -465,7 +541,8 @@ Section proof.
   Qed.
 
   Lemma unseal_spec p γ u v v' φ :
-    {{{ is_unseal γ u φ ∗ is_sealed γ v v' φ }}} u v' @ p; ⊤ {{{ RET v; True }}}.
+    {{{ is_unseal γ u φ ∗ is_sealed γ v v' φ }}} u v' @ p; ⊤
+    {{{ RET v; True }}}.
   Proof.
     iIntros (Φ) "[[#[Hh Hsync] %] Hv'] HΦ". subst. wp_lam.
     wp_apply (wp_alloc_fresh with "Hh"); auto.
@@ -474,7 +551,7 @@ Section proof.
       rewrite/is_sync.
     wp_apply ("Hsync" with "[%]"). iClear "Hsync". iIntros (Ψ) "HR HΨ".
       iDestruct "HR" as (map m) "(Hl & #Hm & Hw & #Hinv)". wp_load.
-      iDestruct (witness_elim with "Hw Hwk") as "%".
+      iDestruct (is_witness_some_elim with "Hw Hwk") as "%".
     wp_apply (map_lookup_partial_Some_spec _ _ _ _ k with "Hm");
       first done. iIntros "_".
     iApply ("HΨ" with "[Hl Hw]").
@@ -489,7 +566,7 @@ Section proof.
     by wp_apply (unseal_body_low with "[$Hctx $Hv'] [$HΦ]").
   Qed.
 
-  Definition sealing : sealing Σ := {|
+  Definition proof : sealing Σ := {|
     intf.seal_low := seal_low;
     intf.unseal_low := unseal_low;
     intf.sealed_low := sealed_low;
@@ -505,9 +582,25 @@ End morris_sealing.
 
 (** * Direct implementation *)
 (**
-	This implemenation supports [strong_unsealing].
+	In contrast to Morris' implementation of sealing, this
+	implemenation supports [strong_unsealing] because low
+	locations are less tricky than low functions.
+
+	With Morris' implementation of sealing, for example, an
+	adversary with values [f1, f2] obtained by sealing values [v1,
+	v2] can construct a function
+<<
+	let r = ref false in
+	λ k,
+	let b := !r in
+	r := (not b);
+	(if b then f1 else f2) k
+>>
+	that, when unsealed, oscillates between [v1] and [v2].
 *)
 Module direct_sealing.
+Import witness.
+
 Section code.
   Context {LI : LockImpl}.
 
@@ -531,25 +624,10 @@ Section code.
   |}.
 End code.
 
-(** The CMRA we need. *)
-Notation heap := (gmap loc val).
-Definition heapUR : ucmraT := gmapUR loc (agreeR valC).
-Class sealingG Σ := SealingG { sealing_heapG :> inG Σ (authR heapUR) }.
-
-Definition sealingΣ : gFunctors := #[ GFunctor (constRF (authR heapUR)) ].
-Instance subG_sealingΣ {Σ} : subG sealingΣ Σ → sealingG Σ.
-Proof. intros [??]%subG_inv. constructor; apply _. Qed.
-
 Section proof.
   Context `{heapG Σ, sealingG Σ, LI : LockImpl} (L : lock Σ).
   Implicit Types l k : loc.
   Implicit Types f v : val.
-
-  Definition is_witness (γ : gname) (k : loc) (v : val) : iProp Σ :=
-    own γ (◯ {[k := to_agree v]}).
-  Definition to_heap : heap → heapUR := fmap to_agree.
-  Definition witness (γ : gname) (m : heap) : iProp Σ :=
-    (own γ (● to_heap m) ∗ live (dom _ m))%I.
 
   Definition tbl_res (l : loc) (γ : gname) (φ : val → iProp Σ) : iProp Σ := (
     ∃ map m, l ↦ map ∗ is_map map m ∗ witness γ m ∗
@@ -582,11 +660,6 @@ Section proof.
 
   (** Structure *)
 
-  Instance is_witness_persistent γ k v : PersistentP (is_witness γ k v).
-  Proof. apply _. Qed.
-  Instance is_witness_timeless γ k v : TimelessP (is_witness γ k v).
-  Proof. apply _. Qed.
-
   Instance tbl_res_ne l γ n : Proper (ext (dist n) ==> dist n) (tbl_res l γ).
   Proof. solve_proper. Qed.
 
@@ -612,69 +685,6 @@ Section proof.
     Proper (ext (dist n) ==> dist n) (is_sealed γ v v').
   Proof. solve_proper. Qed.
 
-  (** Ghosts *)
-
-  Lemma witness_elim γ m k v :
-    witness γ m -∗ is_witness γ k v -∗ ⌜m !! k = Some v⌝.
-  Proof.
-    iIntros "[Hw _] Hk".
-    iDestruct (own_valid_2 with "Hw Hk") as %[Hinc _]%auth_valid_discrete_2.
-    iPureIntro.
-    move: Hinc. rewrite singleton_included lookup_fmap=>-[] u [].
-    case: (m !! k)=>[vh|]/=; last by move=>/option_equivE.
-    move=>Heq. apply (inj Some) in Heq. unfold_leibniz. rewrite -Heq.
-    by case/Some_included=>[/(inj to_agree) | /to_agree_included]->.
-  Qed.
-
-  Lemma witness_alloc' γ m k v :
-    m !! k = None →
-    own γ (● to_heap m) ==∗
-    own γ (● to_heap (<[k:=v]> m)) ∗ is_witness γ k v.
-  Proof.
-    rewrite /to_heap fmap_insert -own_op=>Hdom.
-    apply own_update, auth_update_alloc, alloc_singleton_local_update.
-    by rewrite lookup_fmap Hdom. done.
-  Qed.
-
-  Lemma withness_alloc γ m k v :
-    heap_ctx -∗ witness γ m -∗ fresh k ={⊤}=∗
-    witness γ (<[k:=v]> m) ∗ is_witness γ k v.
-  Proof.
-    iIntros "#Hh [Hw Hlive] Hk".
-    iMod (heap_mark_live with "Hh Hk Hlive") as "(Hdom&Hlive)"; first done.
-      iDestruct "Hdom" as %?%not_elem_of_dom.
-    iMod (witness_alloc' _ _ k v with "Hw") as "[Hw Hv]"; first done.
-    iModIntro. iFrame "Hw Hv". rewrite dom_insert_L. by iFrame "Hlive".
-  Qed.
-
-  Lemma witness_obs γ m k v :
-    m !! k = Some v →
-    witness γ m ==∗ witness γ m ∗ is_witness γ k v.
-  Proof.
-    iIntros (Hdom) "[Hw HL]". rewrite/witness/is_witness. iFrame "HL".
-    rewrite -own_op. iApply (own_update with "Hw").
-    apply auth_frag_alloc; try apply _. apply singleton_included.
-    exists (to_agree v). split. by rewrite lookup_fmap Hdom. done.
-  Qed.
-
-  Lemma witness_agree γ k v1 v2 :
-    is_witness γ k v1 ∗ is_witness γ k v2 ⊢ ⌜v1 = v2⌝.
-  Proof.
-    rewrite -own_op -auth_frag_op.
-    rewrite own_valid auth_validI /= discrete_valid.
-    rewrite op_singleton singleton_valid.
-    by f_equiv=>/agree_op_inv/to_agree_inj/leibniz_equiv_iff.
-  Qed.
-
-  Lemma tbl_inv_insert (m : heap) k v (φ : val → iProp Σ) :
-    ([∗ map] v ∈ m, □ φ v) -∗ □ φ v -∗ [∗ map] v ∈ <[k:=v]> m, □ φ v.
-  Proof.
-    iIntros "Hinv #Hv". case Hv': (m !! k) => [v'|].
-    - rewrite (big_sepM_insert_override_2 _ _ _ v' v) //.
-      iApply "Hinv". iIntros "_". iAlways. by iFrame "Hv".
-    - rewrite big_sepM_insert //. iFrame "Hinv". iAlways. by iFrame "Hv".
-  Qed.
-
   (** Operations *)
 
   Lemma make_seal_spec N p φ :
@@ -683,11 +693,8 @@ Section proof.
     {{{ v1 v2 γ, RET (v1, v2); is_seal γ v1 φ ∗ is_unseal γ v2 φ }}}.
   Proof.
     iIntros (? Φ) "#Hh HΦ". wp_lam. wp_alloc l as "Hl". wp_let.
-      rewrite -wp_fupd. set h := to_heap ∅.
-    iMod (own_alloc (Auth (Excl' h) h)) as (γh) "Hγh"; first done.
-      rewrite (auth_both_op h). iDestruct "Hγh" as "[Hγh _]".
-    iAssert (witness γh ∅) with "[Hγh]" as "Hw".
-    { iFrame "Hγh". by rewrite dom_empty_L big_sepS_empty. }
+      rewrite -wp_fupd.
+    iMod witness_alloc as (γh) "Hw".
     wp_apply (make_sync_spec L _ N (tbl_res l γh φ) with "[$Hh Hl Hw]");
       first done.
     { iExists map_empty, ∅. iFrame "Hl Hw". rewrite big_sepM_empty. by auto. }
@@ -710,7 +717,7 @@ Section proof.
     iIntros "(_&_&_&Hv1) (_&_&_&Hv2)".
     iDestruct "Hv1" as (k1) "[% Hk1]". subst.
     iDestruct "Hv2" as (k2) "[EQ Hk2]". iDestruct "EQ" as %[=<-].
-    by iApply (witness_agree with "[$Hk1 $Hk2]").
+    by iApply (is_witness_agree with "[$Hk1 $Hk2]").
   Qed.
 
   Lemma seal_body p γ v φ :
@@ -725,7 +732,7 @@ Section proof.
     wp_apply ("Hsync" with "[%]"). iIntros (Ψ) "HR HΨ".
       iDestruct "HR" as (map m) "(Hl & #Hm & Hw & #Hinv)". wp_load.
       rewrite -fupd_wp.
-    iMod (withness_alloc _ _ k v with "Hh Hw Hkfresh") as "[Hw Hkv]".
+    iMod (is_witness_alloc _ _ k v with "Hh Hw Hkfresh") as "(%&Hw&Hkv)".
       iModIntro.
     wp_apply (map_insert_spec _ _ _ m with "Hm").
       iIntros (map') "Hm'". wp_store.
@@ -767,11 +774,12 @@ Section proof.
       rewrite/is_sync.
     wp_apply ("Hsync" with "[%]"). iClear "Hsync". iIntros (Ψ) "HR HΨ".
       iDestruct "HR" as (map m) "(Hl & #Hm & Hw & #Hinv)". wp_load.
-      iDestruct (witness_elim with "Hw Hk") as "%".
+      iDestruct (is_witness_elim with "Hw Hk") as "%".
     wp_apply (map_lookup_partial_Some_spec _ _ _ _ k with "Hm")=>//.
       iIntros "_".
-    iApply ("HΨ" with "[Hl Hw]"); last by iApply "HΦ".
-    iExists map, m. by iFrame "Hl Hm Hw Hinv".
+    iApply ("HΨ" with "[Hl Hw]").
+    - iExists map, m. by iFrame "Hl Hm Hw Hinv".
+    - by iApply "HΦ".
   Qed.
 
   Lemma unseal_body_low γ v' φ :
@@ -821,7 +829,7 @@ Section proof.
     iApply "HΦ". by iApply sealed_inv.
   Qed.
 
-  Definition sealing : sealing Σ := {|
+  Definition proof : sealing Σ := {|
     intf.seal_low := seal_low;
     intf.unseal_low := unseal_low;
     intf.sealed_low := sealed_low;
@@ -832,7 +840,6 @@ Section proof.
     intf.unseal_spec := unseal_spec;
     intf.unseal_low_spec := unseal_low_spec
   |}.
-  Global Instance strong : strong_unsealing sealing :=
-    unseal_low_strong.
+  Global Instance strong : strong_unsealing proof := unseal_low_strong.
 End proof.
 End direct_sealing.
